finished HOL_Bindings, added simpproc for assn normalization, adapted proofs

Refine_Imperative_HOL/Sepref_Additional.thy
@@ -2,49 +2,6 @@ theory Sepref_Additional
 imports Sepref_Basic
 begin
 
-
-subsection "Rotate method"
-
-definition gr where "gr A B = A * B"
-
-lemma right_swap: "(A \<Longrightarrow>\<^sub>A B * (C * D)) \<Longrightarrow> (A \<Longrightarrow>\<^sub>A B * (D * C))"
-  by (simp add: assn_times_comm)
-lemma right_take: "(A \<Longrightarrow>\<^sub>A gr B C * D) \<Longrightarrow> (A \<Longrightarrow>\<^sub>A B * (C * D))"
-  by (simp add: gr_def assn_times_assoc) 
-lemma left_swap: "(B * (C * D) \<Longrightarrow>\<^sub>A A) \<Longrightarrow> (B * (D * C) \<Longrightarrow>\<^sub>A A)"
-  by (simp add: assn_times_comm)
-lemma left_take: "(gr B C * D \<Longrightarrow>\<^sub>A A) \<Longrightarrow> (B * (C * D) \<Longrightarrow>\<^sub>A A)"
-  by (simp add: gr_def assn_times_assoc) 
-
-lemma right_move_back: "(A \<Longrightarrow>\<^sub>A B * C) \<Longrightarrow> (A \<Longrightarrow>\<^sub>A C * B)"
-  by (simp add: assn_times_comm)
-lemma left_move_back: "(B * C \<Longrightarrow>\<^sub>A A) \<Longrightarrow> (C * B \<Longrightarrow>\<^sub>A A)"
-  by (simp add: assn_times_comm)
-
-thm mult.assoc
-method rotater = ( (simp only: mult.assoc)? , rule right_move_back , (simp only: mult.assoc)?  )
-method rotatel = ( (simp only: mult.assoc)? , rule left_move_back , (simp only: mult.assoc)?  )
-
-method swapl = ( (simp only: mult.assoc)? ,rule left_swap, (simp only: mult.assoc)?   )
-method takel = ( (simp only: mult.assoc)? , rule left_take, (simp only: mult.assoc)?  )
-
-method swapr = ( (simp only: mult.assoc)? , rule right_swap , (simp only: mult.assoc)?  )
-method taker = ( (simp only: mult.assoc)? , rule right_take, (simp only: mult.assoc)?  )
-
-
-lemma match_first: "A \<Longrightarrow>\<^sub>A B \<Longrightarrow> \<Gamma> * A \<Longrightarrow>\<^sub>A \<Gamma> * B"  
-  by (simp add: assn_times_comm entails_frame)  
-
-lemma match_rest: "emp \<Longrightarrow>\<^sub>A B \<Longrightarrow> \<Gamma> \<Longrightarrow>\<^sub>A \<Gamma> * B"  
-  using match_first by fastforce 
-
-lemma run_and_execute: "(\<forall>\<sigma> t r. run c (Some h) \<sigma> r t \<longrightarrow> \<sigma> \<noteq> None \<and> P (the \<sigma>) r t)
-        \<longleftrightarrow> (\<exists>h' t r. execute c h = Some (r, h', t) \<and> P h' r t)"  
-  apply rule
-  subgoal by (metis option.sel run.intros(2) run.intros(3) timeFrame.elims) 
-  subgoal by (metis (mono_tags) not_None_eq option.sel prod.sel(1) prod.sel(2) run_to_execute) 
-  done
-
 lemma hoare_alt: 
   "<P> c <\<lambda>r. Q r > = (\<forall>h as n.
         pHeap h as n \<Turnstile> P \<longrightarrow> (\<exists>h' t r. execute c h = Some (r, h', t) \<and>
@@ -89,7 +46,7 @@ proof -
     from h assms(3) have h': "pHeap h' (new_addrs h as h') (n + Cost_lb - t) \<Turnstile>   \<Gamma>' * (\<exists>\<^sub>Ara. R ra r * \<up> (ra \<in> dom M)) * true"
       by (simp add: entails_def)
     then have "\<exists>ra. pHeap h' (new_addrs h as h') (n + Cost_lb - t) \<Turnstile>   \<Gamma>' *  R ra r * \<up> (ra \<in> dom M) * true"
-      by(simp add: ex_distrib_star' ex_distrib_star[symmetric] mod_ex_dist assn_times_assoc)
+      by simp
     then obtain ra where h'': "pHeap h' (new_addrs h as h') (n + Cost_lb - t) \<Turnstile>   \<Gamma>' *  R ra r * \<up> (ra \<in> dom M) * true"
         by blast
     have "pHeap h' (new_addrs h as h') (n + Cost_lb - t) \<Turnstile>   (\<Gamma>' *  R ra r * true) * \<up> (ra \<in> dom M)"
@@ -193,8 +150,7 @@ proof (goal_cases)
     subgoal using H by simp  
     subgoal by fact
      apply fact apply fact done
-qed
-
-
+qed 
+     
 
 end
